tests/fin_maps.v
@@ -378,12 +378,12 @@ Proof.
   intros Hnode t.
   remember (gtest_size t) as n eqn:Hn. revert t Hn.
   induction (lt_wf n) as [n _ IH]; intros [ts] ->; simpl in *.
-  apply Hnode. induction ts as [|k t m ? Hfold IHm] using map_first_key_ind.
-  - apply map_Forall_empty.
-  - apply map_Forall_insert; [done|]. split.
-    + eapply IH; [|done]. rewrite map_fold_insert_first_key by done. lia.
-    + eapply IHm. intros; eapply IH; [|done].
-      rewrite map_fold_insert_first_key by done. lia.
+  apply Hnode. revert ts IH.
+  apply (map_fold_ind (λ r ts, (∀ n', n' < S r → _) → map_Forall (λ _, P) ts)).
+  - intros IH. apply map_Forall_empty.
+  - intros k t m r ? IHm IHt. apply map_Forall_insert; [done|]. split.
+    + eapply IHt; [|done]; lia.
+    + eapply IHm. intros; eapply IHt;[|done]; lia.
 Qed.
 
 (** We show that [gtest K] is countable itself. This means that we can use
@@ -415,11 +415,12 @@ Global Program Instance gtest_countable `{Countable K} : Countable (gtest K) :=
   inj_countable' enc dec _.
 Next Obligation.
   intros K ?? enc dec_list dec t.
-  induction (Nat.lt_wf_0_projected gtest_size t) as [[ts] _ IH]. f_equal/=.
-  induction ts as [|i t ts ? Hfold IHts] using map_first_key_ind; [done|].
-  rewrite map_fold_insert_first_key by done. f_equal/=.
-  - eapply IH. rewrite map_fold_insert_L by auto with lia. lia.
-  - apply IHts; intros t' ?. eapply IH.
+  induction (Nat.lt_wf_0_projected gtest_size t) as [[ts] _ IH].
+  simpl in *; f_equal.
+  revert ts IH. apply (map_fold_ind (λ r ts, _ → dec_list dec r = ts)); [done|].
+  intros i t ts r ? IHts IHt; simpl. f_equal.
+  - eapply IHt. rewrite map_fold_insert_L by auto with lia. lia.
+  - apply IHts; intros t' ?. eapply IHt.
     rewrite map_fold_insert_L by auto with lia. lia.
 Qed.
 
@@ -433,9 +434,3 @@ Proof. discriminate. Qed.
 
 Goal GTest {[ GTest {[ 1 := GTest ∅ ]} := GTest ∅ ]} ≠@{gtest (gtest nat)} GTest ∅.
 Proof. discriminate. Qed.
-
-(* Test that a fixpoint can be recursively invoked in the closure argument
-of [map_imap]. *)
-Fixpoint gtest_imap `{Countable K} (j : K) (t : gtest K) : gtest K :=
-  let '(GTest ts) := t in
-  GTest (map_imap (λ i t, guard (i = j);; Some (gtest_imap j t)) ts).
